intm/CompCertSem.v
@@ -1,0 +1,148 @@
+Require Import LogicalRelations.
+Require Import KLR.
+Require Import Axioms.
+Require Import Errors.
+Require Import LanguageInterface.
+Require Import Smallstep.
+Require Import SmallstepInteraction.
+Require Import Clight.
+Require Import Asm.
+Require Import Compiler.
+Require Import IntmDef.
+Require Import IntmTactics.
+Require Import IntmIter.
+Require Import IntmDecomp.
+Require Import IntmAbs.
+
+Import IntmDef.Behavior.
+Import IntmIter.Behavior.
+Import IntmAbs.Behavior.
+
+
+(** * Semantic domains *)
+
+Definition zero {li} : sem li :=
+  fun q => bot.
+
+Definition plus {li} (σ1 σ2 : sem li) : sem li :=
+  fun q => join (σ1 q) (σ2 q).
+
+Lemma plus_assoc {li} (σ1 σ2 σ3 : sem li) :
+  plus (plus σ1 σ2) σ3 = plus σ1 (plus σ2 σ3).
+Proof.
+  apply functional_extensionality.
+  unfold plus. monad.
+Qed.
+
+Lemma plus_comm {li} (σ1 σ2 : sem li) :
+  plus σ1 σ2 = plus σ2 σ1.
+Proof.
+  apply functional_extensionality.
+  unfold plus. monad.
+Qed.
+
+Lemma plus_zero_l {li} (σ : sem li) :
+  plus zero σ = σ.
+Proof.
+  apply functional_extensionality.
+  unfold plus, zero. monad.
+Qed.
+
+Lemma plus_zero_r {li} (σ : sem li) :
+  plus σ zero = σ.
+Proof.
+  apply functional_extensionality.
+  unfold plus, zero. monad.
+Qed.
+
+Infix "+" := plus : behavior_scope.
+Notation "0" := zero : behavior_scope.
+
+Global Instance plus_ccsim :
+  Monotonic
+    (@plus)
+    (forallr cc : flip callconv, ccsim cc ++> ccsim cc ++> ccsim cc).
+Proof.
+  unfold plus, ccsim.
+  repeat rstep.
+  - eapply H; eauto.
+  - eapply H0; eauto.
+Qed.
+
+
+(** * CompCert compilation unit semantics *)
+
+Global Instance clight_sem : Semof li_c Clight.program :=
+  {
+    semof p := 〚Clight.semantics2 p〛;
+  }.
+
+Global Instance asm_sem : Semof li_asm Asm.program :=
+  {
+    semof p := 〚Asm.semantics p〛;
+  }.
+
+Lemma compcert_correct (p : Clight.program) (tp : Asm.program) :
+  transf_clight_program p = OK tp ->
+  ccsim cc_compcert 〚tp〛 〚p〛.
+Proof.
+  intros H.
+  apply transf_clight_program_correct in H.
+  destruct H.
+  eapply soundness; eauto.
+Qed.
+
+
+(** * Multi-module semantics *)
+
+Require Import List.
+Local Open Scope behavior_scope.
+
+(** ** Definition *)
+
+Global Instance mmsem `(Semof) : Semof li (list P) :=
+  {
+    semof :=
+      fold_right (fun p x => 〚p〛 + x) 0;
+  }.
+
+Lemma mmsem_app `{Semof} (p1 p2 : list P) :
+  〚p1 ++ p2〛 = 〚p1〛 + 〚p2〛.
+Proof.
+  induction p1; eauto.
+  - cbn.
+    rewrite plus_zero_l.
+    reflexivity.
+  - cbn in *.
+    rewrite IHp1, plus_assoc.
+    reflexivity.
+Qed.
+
+(** ** Multi-module compiler *)
+
+Definition mmcompcert : list Clight.program -> res (list Asm.program) :=
+  fold_right
+    (fun p r =>
+       match r, transf_clight_program p with
+         | OK ltp, OK tp => OK (tp :: ltp)
+         | Error msg, _ => Error msg
+         | _, Error msg => Error msg
+       end)
+    (OK nil).
+
+Lemma mmcompcert_correct lp ltp :
+  mmcompcert lp = OK ltp ->
+  ccsim cc_compcert 〚ltp〛 〚lp〛.
+Proof.
+  revert ltp. induction lp as [ | p lp IHlp].
+  - inversion 1; clear H; subst. cbn.
+    unfold ccsim, zero, sim. repeat rstep. monad.
+  - intros ltp Hltp.
+    cbn in *.
+    destruct mmcompcert as [xltp|msg] eqn:Hxltp; try congruence.
+    destruct transf_clight_program as [tp|msg] eqn:Htp; try congruence.
+    inversion Hltp; clear Hltp; subst. cbn.
+    unfold ccsim, plus. do 5 rstep.
+    + apply compcert_correct; eauto.
+    + apply IHlp; eauto.
+Qed.
